logrel_intrinsic: eval, log. rel and fundamental lemmata sketch

logrel/logrel_intrinsic.v
@@ -14,10 +14,10 @@ Import ListNotations.
   Compatible with Coq 8.12.1.
 
   TODOs
-  * fix the self-references in the recursive types
   * equality for types
   * evaluator on intrinsically-scoped syntax
   * logrel and sn proofs
+  * add and fix the self-references in the recursive types
 *)
 
 
@@ -43,14 +43,14 @@ Inductive ty : nat -> Type :=
 | TAll  : forall {n}, ty n -> ty (S n) -> ty n
 | TSel  : forall {n}, tm n -> ty n
 | TMem  : forall {n}, ty n -> ty n -> ty n
-| TBind : forall {n}, ty (S n)  -> ty n
+(* | TBind : forall {n}, ty (S n)  -> ty n *)
 | TAnd  : forall {n}, ty n -> ty n -> ty n
 with tm : nat -> Type :=
 | tvar    : forall {n}, var n -> tm n
 | ttyp    : forall {n}, ty n -> tm n
 | tabs    : forall {n}, ty n -> tm (S n) -> tm n
 | tapp    : forall {n}, tm n -> tm n -> tm n
-| tunpack : forall {n}, tm n -> tm (S n) -> tm n
+(* | tunpack : forall {n}, tm n -> tm (S n) -> tm n *)
 .
 
 
@@ -85,7 +85,7 @@ Fixpoint ren_ty {n m} (ρ : Ren n m) (T : ty n): ty m :=
   | TAll  T1 T2, ρ => TAll  (ren_ty ρ T1) (ren_ty (lift ρ) T2)
   | TSel  t    , ρ => TSel  (ren_tm ρ t)
   | TMem  T1 T2, ρ => TMem  (ren_ty ρ T1) (ren_ty ρ T2)
-  | TBind T    , ρ => TBind (ren_ty (lift ρ) T)
+  (* | TBind T    , ρ => TBind (ren_ty (lift ρ) T) *)
   | TAnd  T1 T2, ρ => TAnd  (ren_ty ρ T1) (ren_ty ρ T2)
   end
 with ren_tm {n m} (ρ : Ren n m) (t : tm n) : tm m :=
@@ -94,7 +94,7 @@ with ren_tm {n m} (ρ : Ren n m) (t : tm n) : tm m :=
   | ttyp    T    , ρ => ttyp    (ren_ty ρ T)
   | tabs    T  t , ρ => tabs    (ren_ty ρ T)  (ren_tm (lift ρ) t)
   | tapp    t1 t2, ρ => tapp    (ren_tm ρ t1) (ren_tm ρ t2)
-  | tunpack t1 t2, ρ => tunpack (ren_tm ρ t1) (ren_tm (lift ρ) t2)
+  (* | tunpack t1 t2, ρ => tunpack (ren_tm ρ t1) (ren_tm (lift ρ) t2) *)
   end.
 
 Definition weaken_tm {n} (t : tm n): tm (S n) := ren_tm (FS n) t.
@@ -138,7 +138,7 @@ Fixpoint sub_tm {n m} (σ : Sub n m) (t : tm n) : tm m :=
   | ttyp    T    , σ => ttyp    (sub_tm_ty σ T)
   | tabs    T  t , σ => tabs    (sub_tm_ty σ T) (sub_tm (lifts σ) t)
   | tapp    t1 t2, σ => tapp    (sub_tm σ t1)   (sub_tm σ t2)
-  | tunpack t1 t2, σ => tunpack (sub_tm σ t1)   (sub_tm (lifts σ) t2)
+  (* | tunpack t1 t2, σ => tunpack (sub_tm σ t1)   (sub_tm (lifts σ) t2) *)
   end
 with
 sub_tm_ty {n m} (σ : Sub n m) (T : ty n) : ty m :=
@@ -148,22 +148,22 @@ sub_tm_ty {n m} (σ : Sub n m) (T : ty n) : ty m :=
   | TAll  T1 T2, σ => TAll  (sub_tm_ty σ T1) (sub_tm_ty (lifts σ) T2)
   | TSel  t    , σ => TSel  (sub_tm σ t)
   | TMem  T1 T2, σ => TMem  (sub_tm_ty σ T1) (sub_tm_ty σ T2)
-  | TBind T    , σ => TBind (sub_tm_ty (lifts σ) T)
+  (* | TBind T    , σ => TBind (sub_tm_ty (lifts σ) T) *)
   | TAnd  T1 T2, σ => TAnd  (sub_tm_ty σ T1) (sub_tm_ty σ T2)
   end.
 
 Definition sub1_tm    {n} (this : tm n) (there : tm (S n)) : tm n := sub_tm    (extend tvar this) there.
 Definition sub1_tm_ty {n} (this : tm n) (there : ty (S n)) : ty n := sub_tm_ty (extend tvar this) there.
 
-Notation "⟨ t1 <~ t2 ⟩"  := (sub1_tm t2 t1) (at level 75).
-Notation "⟪ t1 <~ t2 ⟫" := (sub1_tm_ty t2 t1) (at level 75).
+Notation "t1 <~ t2"  := (sub1_tm t2 t1) (at level 75).
+Notation "t1 <*~ t2" := (sub1_tm_ty t2 t1) (at level 75).
 
 (* valid expressions that may appear in type selections *)
 Inductive wf_tsel : forall {n : nat}, tm n -> Prop :=
 | wf_tsel_var : forall {n} (x : var n), wf_tsel (tvar x)
-| wf_tsel_typ : forall {n} (T : ty n), wf_tsel (ttyp T) (*FIXME: should we also check that T is well-formed? *)
-| wf_tsel_app : forall {n} (t1 t2 : tm n), wf_tsel t1 -> wf_tsel t2 -> wf_tsel (tapp t1 t2)
-| wf_tsel_lam : forall {n} (T : ty n) (t : tm (S n)), wf_tsel t -> wf_tsel (tabs T t) (*FIXME: should we also check that T is well-formed? *)
+(* | wf_tsel_typ : forall {n} (T : ty n), wf_tsel (ttyp T) (*FIXME: should we also check that T is well-formed? *) *)
+(* | wf_tsel_app : forall {n} (t1 t2 : tm n), wf_tsel t1 -> wf_tsel t2 -> wf_tsel (tapp t1 t2) *)
+(* | wf_tsel_lam : forall {n} (T : ty n) (t : tm (S n)), wf_tsel t -> wf_tsel (tabs T t) (*FIXME: should we also check that T is well-formed? *) *)
 .
 
 Inductive has_type : forall {n : nat}, tenv n -> tm n -> ty n -> Prop :=
@@ -186,16 +186,16 @@ Inductive has_type : forall {n : nat}, tenv n -> tm n -> ty n -> Prop :=
     has_type Γ t1 (TAll T1 T2) ->
     has_type Γ t2 T1 ->
     wf_tsel t2 ->
-    has_type Γ (tapp t1 t2) (⟪ T2 <~ t2 ⟫)
+    has_type Γ (tapp t1 t2) (T2 <*~ t2)
 
 | t_and : forall {n} (Γ : tenv n) (x : var n) (T1 T2 : ty n),
     has_type Γ (tvar x) T1 ->
     has_type Γ (tvar x) T2 ->
     has_type Γ (tvar x) (TAnd T1 T2)
 
-| t_var_pack : forall {n} (Γ : tenv n) (x : var n) (T : ty (S n)),
-    has_type Γ (tvar x) (⟪ T <~ (tvar x) ⟫) -> (* FIXME: how to express self-reference in the intrinsically-scoped style? *)
-    has_type Γ (tvar x) (TBind T)
+(* | t_var_pack : forall {n} (Γ : tenv n) (x : var n) (T : ty (S n)), *)
+(*     has_type Γ (tvar x) (T <*~ (tvar x)) -> (* FIXME: how to express self-reference in the intrinsically-scoped style? *) *)
+(*     has_type Γ (tvar x) (TBind T) *)
 
 (* FIXME: how to express self-reference in the intrinsically-scoped style? have second sort of variable? *)
 (* | t_unpack : forall {n} (Γ : tenv n) (t1 : tm n) (t2 : tm (S n)) (T1: ty (S n)) (T2 : ty n), *)
@@ -270,3 +270,234 @@ with stp : forall {n : nat}, tenv n -> ty n -> ty n -> Prop :=
 .
 
 (* TODO type equality! *)
+
+Lemma lift_id : forall {n} {v : var (S n)}, lift id v = v.
+Proof.
+  intros. dependent destruction v; eauto.
+Qed.
+
+Open Scope program_scope.
+Lemma lift_comp : forall {n m k} {ρ : Ren n m} {ρ' : Ren m k} {v : var (S n)}, lift (ρ' ∘ ρ) v = lift ρ' (lift ρ v).
+Proof.
+  intros. dependent destruction v; eauto.
+Qed.
+
+(* Lemma substitution : forall {n} {Γ : tenv n} {T1 : ty n} {T2 : ty (S n)}  {t : tm (S n)}, *)
+(*     has_type (Γ ;; T1) t T2 -> forall {t' : tm n}, has_type Γ t' T1 -> has_type Γ (t <~ t') (T2 <*~ t'). *)
+(* Proof. *)
+(*   intros n Γ T1 T2 t Hty. *)
+(*   dependent induction Hty; intros. *)
+(*   - admit. *)
+(*   - unfold sub1_tm. unfold sub1_tm_ty. simpl. constructor. *)
+(*   - unfold sub1_tm in *. unfold sub1_tm_ty in *. simpl. constructor. *)
+(*     admit. *)
+(*   - unfold sub1_tm. unfold sub1_tm_ty. *)
+
+Inductive env (T : Type) : nat -> Type :=
+| enil  : env T 0
+| econs : forall{n}, env T n -> T -> env T (S n)
+.
+Arguments econs {T n}.
+Arguments enil {T}.
+
+Inductive vl : Type :=
+| vabs : forall {n : nat}, env vl n -> tm (S n) -> vl
+| vty :  forall {n : nat}, env vl n -> ty n -> vl
+.
+
+Definition venv := env vl.
+
+Variable get : forall { T : Type } {n : nat}, env T n -> var n -> T.
+
+Inductive Result : Type :=
+| Done   : vl -> Result
+| Error  : Result
+| NoFuel : Result
+.
+
+Fixpoint eval{m : nat}(fuel : nat)(γ : venv m)(t : tm m){struct fuel}: Result :=
+  match fuel with
+  | 0   => NoFuel
+  | S n =>
+    match t, γ with
+    | tvar x, γ => Done (get γ x)
+    | ttyp T, γ    => Done (vty γ T)
+    | tabs T t, γ  => Done (vabs γ t)
+    | tapp t1 t2, γ =>
+      match eval n γ t2 with
+      | Done v2 =>
+        match eval n γ t1 with
+        | Done (vabs γ' t) => eval n (econs γ' v2) t
+        | Done _  => Error
+        | err => err
+        end
+      | err => err
+      end
+    (* | tunpack t1 t2 => *)
+    (*   match eval n γ t1 with *)
+    (*   | Done v1 => eval n (v1 :: γ) t2 *)
+    (*   | err => err *)
+    (*   end *)
+    end
+  end.
+
+Fixpoint vset (n : nat): Type := match n with
+                               | 0 => vl -> Prop
+                               | S n => vset n -> vl -> Prop
+                               end.
+
+Definition vseta  := forall n, vset n.
+
+Notation Dom := vseta.
+
+Definition denv := env Dom.
+
+(* vseta membership *)
+Definition vseta_mem (v:vl) (vs1: vseta) (vs2: vseta): Prop :=
+  forall n, vs2 (S n) (vs1 n) v.
+Notation "⦑ x , y ⦒ ⋵ vs" := (vseta_mem x y vs) (at level 79).
+
+Definition elem2 {A B} (γ : A) (v : B) (P : A -> B -> Prop) := P γ v.
+Notation "⟨ H , v ⟩ ∈ D" := (elem2 H v D) (at level 75).
+Hint Unfold elem2 : dsub.
+
+(* Subset relation for use in comprehensions with explicit index parameter *)
+Definition vset_sub_eq {n:nat}: vset n -> vset n -> Prop :=
+  match n with
+       | 0 => fun vs1 vs2 => True
+       | S n => fun vs1 vs2 => forall vs' v, (vs1 vs' v) -> (vs2 vs' v)
+       end.
+
+(* Subset relation closing over all n, for use in the vesta lattice, e.g., monotonicity check*)
+Definition vseta_sub_eq (vs1: vseta) (vs2: vseta) :=
+  forall n, vset_sub_eq (vs1 n) (vs2 n).
+
+Hint Unfold vset_sub_eq : dsub.
+Hint Unfold vseta_sub_eq : dsub.
+
+(* \sqsubseteq *)
+Notation "vs1 ⊑# vs2" := (vset_sub_eq vs1 vs2) (at level 75).
+Notation "vs1 ⊑  vs2" := (vseta_sub_eq vs1 vs2) (at level 75).
+
+(* vseta comprehension exposing the index in the body *)
+Notation "{{ ' p vs n | P }}" := (fun k =>
+                                   match k with
+                                   | 0   => fun _ => True
+                                   | S n => fun (vs : vset n) (v : vl) =>
+                                              match v with
+                                              | p => P
+                                              | _ => False
+                                              end
+                                   end)
+                              (at level 0, p pattern, vs ident, n ident ).
+
+Notation "{{ v vs n | P }}" := (fun k =>
+                                   match k with
+                                   | 0   => fun _ => True
+                                   | S n => fun (vs : vset n) (v : vl) => P
+                                   end)
+                              (at level 0, v ident, vs ident, n ident ).
+
+
+(* The domain vseta is a complete lattice, which we require for least and greatest fixpoints of types. *)
+Definition vseta_top: vseta := {{ v vs n | True }}.
+
+Definition vseta_bot: vseta := {{ v vs n | False }}.
+
+Definition vseta_join (vs1: vseta) (vs2: vseta): vseta := {{ v vs n | (vs1 (S n) vs v) \/ (vs2 (S n) vs v) }}.
+(* \sqcup *)
+Notation "vs1 ⊔ vs2" := (vseta_join vs1 vs2) (at level 70, right associativity).
+
+Definition vseta_meet (vs1: vseta) (vs2: vseta): vseta := {{ v vs n | (vs1 (S n) vs v) /\ (vs2 (S n) vs v) }}.
+(* \sqcap *)
+Notation "vs1 ⊓ vs2" := (vseta_meet vs1 vs2) (at level 65, right associativity).
+
+Lemma subset_refl : forall X, X ⊑ X.
+Proof.
+  intros. unfold vseta_sub_eq. unfold vset_sub_eq. intros.
+  induction n; eauto.
+Qed.
+Hint Resolve subset_refl : dsub.
+
+Lemma subset_trans : forall {X Y Z}, X ⊑ Y -> Y ⊑ Z -> X ⊑ Z.
+Proof.
+  intros. unfold vseta_sub_eq in *. induction n.
+  - specialize (H 0). specialize (H0 0). simpl. eauto.
+  - simpl. intros. specialize (H (S n)). specialize (H0 (S n)).
+    eauto.
+Qed.
+
+Lemma subset'_refl : forall {n} {X : vset n}, X ⊑# X.
+Proof.
+  intros. unfold vset_sub_eq.
+  induction n; eauto.
+Qed.
+Hint Resolve subset'_refl : dsub.
+
+Lemma subset'_trans : forall {n} {X Y Z : vset n}, X ⊑# Y -> Y ⊑# Z -> X ⊑# Z.
+Proof.
+  intros. unfold vset_sub_eq in *. induction n; eauto.
+Qed.
+
+Definition ℰ {m : nat} (D : Dom) (γ : venv m) (t : tm m) : Prop :=
+  exists k v, eval k γ t = Done v /\ exists vs, ⦑ v, vs ⦒ ⋵ D.
+
+Fixpoint val_type {m : nat} (T : ty m) (ρ : denv m) : Dom :=
+  match T , ρ with
+  | TTop, _          => vseta_top
+  | TAll T1 T2, ρ    =>
+     {{ '(vabs γ t) D n | forall vx Dx, ⦑ vx, Dx ⦒ ⋵ (val_type T1 ρ) ->
+                                  ⟨ (econs γ vx) , t  ⟩ ∈ ℰ (val_type T2 (econs ρ Dx))  }}
+  | TSel (tvar x), ρ => get ρ x
+  | TMem T1 T2, ρ    =>
+    {{ '(vty γ T) D n | (val_type T1 ρ n) ⊑# D /\ D ⊑# (val_type T2 ρ n) }}
+  | TAnd T1 T2 , ρ   => (val_type T1 ρ) ⊓ (val_type T2 ρ)
+  | _ , _            => vseta_bot (* we only have this case because we allow arbitrary t in TSel *)
+  end.
+
+
+Inductive 𝒞𝓉𝓍 : forall {n : nat}, (tenv n) -> (denv n) -> (venv n) -> Prop :=
+| 𝒞𝓉𝓍_nil :
+    𝒞𝓉𝓍 (vnil ty) enil enil
+| 𝒞𝓉𝓍_cons : forall {n : nat } {Γ : tenv n} {ρ : denv n} { γ : venv n } {T : ty n} {v D},
+    𝒞𝓉𝓍 Γ ρ γ  ->
+    ⦑ v, D ⦒ ⋵ (val_type T ρ) ->
+    𝒞𝓉𝓍 (Γ ;; T) (econs ρ D) (econs γ v)
+.
+
+Lemma fundamental     : (forall {n : nat} {Γ : tenv n} {t : tm n} {T : ty n}, has_type Γ t T -> forall{ρ : denv n} {γ : venv n}, 𝒞𝓉𝓍 Γ ρ γ -> ⟨ γ , t ⟩ ∈ ℰ (val_type T ρ))
+with  fundamental_stp : (forall {n : nat} {Γ : tenv n} {S T : ty n}, stp Γ S T -> forall{ρ : denv n} {γ : venv n}, 𝒞𝓉𝓍 Γ ρ γ -> (val_type S ρ) ⊑ (val_type T ρ)).
+Proof.
+  - clear fundamental. intros m Γ t T Hty. dependent induction Hty; intros ρ γ HΓργ; unfold ℰ in *; unfold elem2 in *.
+    + (* t_var *)
+      exists 1. exists (get γ x). intuition. exists (get ρ x). admit. (* TODO this is exactly a reasonable lookup lemma *)
+    + (* t_typ *)
+      exists 1. exists (vty γ T). intuition. exists (val_type T ρ). unfold vseta_mem.
+      intros m. simpl. split; apply subset'_refl.
+    + (* t_abs *)
+      exists 1. exists (vabs γ t). intuition. exists vseta_top. unfold vseta_mem.
+      intros m. simpl. intros.
+      assert (Hext: 𝒞𝓉𝓍 (Γ;; T1) (econs ρ Dx) (econs γ vx)) by (constructor; eauto).
+      apply IHHty in Hext. destruct Hext as [k [vy [Heval [vsy vyvsyT2 ]]]].
+      unfold elem2. unfold ℰ. exists k. exists vy. intuition. exists vsy. auto.
+    + (* t_app *)
+      specialize (IHHty1 _ _ HΓργ). specialize (IHHty2 _ _ HΓργ).
+      destruct IHHty1 as [k1 [v1 [evalv1 [vs1 v1vs1inVtyT1T2 ]]]].
+      destruct IHHty2 as [k2 [v2 [evalv2 [vs2 v2vs2inVtyT1]]]].
+      specialize (v1vs1inVtyT1T2 0). simpl in v1vs1inVtyT1T2.
+      destruct v1 as [ i γ' t' | i γ' T' ]; intuition.
+      apply v1vs1inVtyT1T2 in v2vs2inVtyT1. unfold elem2 in *. unfold ℰ in *.
+      destruct v2vs2inVtyT1 as [k3 [v3 [evalapp [vs3 v3vs3inVtyT2] ]]].
+      exists (k1 + k2 + k3). exists v3. split. admit. (* TODO: need to show monotonicity of eval *)
+      exists vs3. admit. (* that should be a relatively easy lemma *)
+    + (* t_dapp *)
+      specialize (IHHty1 _ _ HΓργ). specialize (IHHty2 _ _ HΓργ).
+      destruct IHHty1 as [k1 [v1 [evalv1 [vs1 v1vs1inVtyT1T2 ]]]].
+      destruct IHHty2 as [k2 [v2 [evalv2 [vs2 v2vs2inVtyT1]]]].
+      specialize (v1vs1inVtyT1T2 0). simpl in v1vs1inVtyT1T2.
+      destruct v1 as [ i γ' t' | i γ' T' ]; intuition.
+      apply v1vs1inVtyT1T2 in v2vs2inVtyT1. unfold elem2 in *. unfold ℰ in *.
+      destruct v2vs2inVtyT1 as [k3 [v3 [evalapp [vs3 v3vs3inVtyT2] ]]].
+      exists (k1 + k2 + k3). exists v3. split. admit. (* TODO: need to show monotonicity of eval *)
+      exists vs3. (* TODO: this one is trickier, maybe first do the original system with single variables in selections? *)
+Admitted.
